compiler/backend/proofs/source_lift_constsProofScript.sml
@@ -1,0 +1,36 @@
+(*
+  Correctness for the source_lift_consts passes.
+ *)
+
+open preamble astTheory evaluateTheory evaluatePropsTheory
+     semanticPrimitivesTheory semanticPrimitivesPropsTheory
+     semanticsTheory source_lift_constsTheory source_evalProofTheory;
+
+val _ = new_theory "source_lift_constsProof";
+
+val _ = set_grammar_ancestry
+  [ "source_lift_consts", "evaluate", "evaluateProps", "semanticPrimitives",
+    "semanticPrimitivesProps", "misc", "semantics" ];
+
+Theorem compile_semantics:
+  ¬semantics_prog s env prog Fail ∧
+  semantics_prog s env prog outcome ⇒
+    semantics_prog s env (compile_decs prog) outcome
+Proof
+  cheat
+QED
+
+Theorem compile_semantics_oracle:
+  ∀f.
+    source_evalProof$is_insert_oracle ci f s.eval_state ∧
+    ¬ semantics_prog s env prog Fail ∧
+    semantics_prog s env prog outcome
+    ⇒
+    semantics_prog (s with eval_state updated_by
+              source_evalProof$adjust_oracle ci (compile_decs ∘ f))
+          env prog outcome
+Proof
+  cheat
+QED
+
+val _ = export_theory ();
