compiler/backend/proofs/source_to_sourceProofScript.sml
@@ -4,28 +4,63 @@
 
 open preamble astTheory evaluateTheory evaluatePropsTheory
      semanticPrimitivesTheory semanticPrimitivesPropsTheory
-     semanticsTheory source_to_sourceTheory source_letProofTheory
+     semanticsTheory source_to_sourceTheory semanticsPropsTheory
+     source_letProofTheory
+     source_lift_constsProofTheory
      source_evalProofTheory;
 
 val _ = new_theory "source_to_sourceProof";
 
-val _ = set_grammar_ancestry [
-  "source_letProof", "source_to_source", "evaluate", "evaluateProps",
-  "semanticPrimitives", "semanticPrimitivesProps", "misc", "semantics"
-  ];
+val _ = set_grammar_ancestry
+  [ "source_letProof", "source_lift_constsProof",
+    "source_to_source", "evaluate", "evaluateProps",
+    "semanticPrimitives", "semanticPrimitivesProps", "misc", "semantics" ];
+
+Triviality semantics_prog_11:
+  semantics_prog s env prog outcome1 ∧
+  semantics_prog s env prog outcome2 ⇒
+  outcome1 = outcome2
+Proof
+  metis_tac [semanticsPropsTheory.semantics_prog_deterministic]
+QED
 
 Theorem compile_semantics:
   ¬semantics_prog s env prog Fail ∧
   semantics_prog s env prog outcome ⇒
     semantics_prog s env (compile prog) outcome
 Proof
-  rw [compile_def]
-  \\ irule source_letProofTheory.compile_semantics
-  \\ gs []
+  rw [source_to_sourceTheory.compile_def]
+  \\ drule_all source_letProofTheory.compile_semantics
+  \\ strip_tac
+  \\ drule_at Any source_lift_constsProofTheory.compile_semantics
+  \\ impl_tac
+  >-
+   (strip_tac
+    \\ imp_res_tac semantics_prog_11
+    \\ rpt var_eq_tac \\ fs [])
+  \\ fs [semantics_prog_def]
+QED
+
+Triviality adjust_oracle_o:
+  source_evalProof$adjust_oracle cj f ∘
+  source_evalProof$adjust_oracle ci g =
+  source_evalProof$adjust_oracle cj f
+Proof
+  fs [adjust_oracle_def,FUN_EQ_THM]
+  \\ Cases \\ fs []
+  \\ Cases_on ‘x'’ \\ fs []
+QED
+
+Triviality compile_eq:
+  source_to_source$compile =
+    source_lift_consts$compile_decs o
+    source_let$compile_decs
+Proof
+  fs [FUN_EQ_THM,source_to_sourceTheory.compile_def]
 QED
 
 Theorem compile_semantics_oracle:
-  !f.
+  ∀f.
   source_evalProof$is_insert_oracle ci f s.eval_state ∧
   ¬ semantics_prog s env prog Fail ∧
   semantics_prog s env prog outcome ⇒
@@ -33,11 +68,24 @@ Theorem compile_semantics_oracle:
             source_evalProof$adjust_oracle ci (compile ∘ f))
         env prog outcome
 Proof
-  rw [compile_def]
-  \\ irule source_letProofTheory.compile_semantics_oracle
-  \\ simp []
+  rw [source_to_sourceTheory.compile_def]
+  \\ drule_all source_letProofTheory.compile_semantics_oracle
+  \\ strip_tac
+  \\ drule_at (Pos last) source_lift_constsProofTheory.compile_semantics_oracle
+  \\ fs [adjust_oracle_o,compile_eq]
+  \\ disch_then irule
+  \\ conj_tac
+  >-
+   (strip_tac
+    \\ imp_res_tac semantics_prog_11
+    \\ rpt var_eq_tac \\ fs [])
+  \\ last_x_assum mp_tac
+  \\ fs [is_insert_oracle_def,adjust_oracle_def]
+  \\ rw [] \\ fs []
+  \\ fs [insert_gen_oracle_def]
+  \\ every_case_tac
+  \\ fs [AllCaseEqs()]
+  \\ metis_tac []
 QED
 
-
 val _ = export_theory ();
-
