compiler/backend/README.md
@@ -262,6 +262,10 @@ Proofs and automation for serialising HOL values.
 This is a source-to-source transformation that lifts Let/Letrec expressions
 that sit at the top of Dlet:s into their own Dlet/Dletrec:s.
 
+[source_lift_constsScript.sml](source_lift_constsScript.sml):
+This is a source-to-source transformation that lifts constants
+from within function expressions to top-level local-declarations.
+
 [source_to_flatScript.sml](source_to_flatScript.sml):
 This is the compiler phase that translates the CakeML source
 language into flatLang.
