compiler/backend/proofs/README.md
@@ -124,6 +124,9 @@ be switched to one that includes an oracle.
 [source_letProofScript.sml](source_letProofScript.sml):
 Correctness for the source_let pass.
 
+[source_lift_constsProofScript.sml](source_lift_constsProofScript.sml):
+Correctness for the source_lift_consts passes.
+
 [source_to_flatProofScript.sml](source_to_flatProofScript.sml):
 Correctness proof for source_to_flat
 
